#192 done

abp/SenderAutomaton.thy
@@ -3,7 +3,7 @@
  * This file was generated from Sender.maa and will be overridden when changed. To change
  * permanently, consider changing the model itself.
  *
- * Generated on Sep 5, 2018 3:18:21 PM by isartransformer 1.0.0
+ * Generated on Sep 18, 2018 2:23:42 PM by isartransformer 1.0.0
  *)
 theory SenderAutomaton
   imports bundle.tsynBundle automat.dAutomaton
@@ -36,23 +36,23 @@ end
 
 section \<open>Helpers to create a bundle from a single raw element\<close>
 
-lift_definition createAsBundle :: "bool \<Rightarrow> senderMessage tsyn SB" is
-"\<lambda>x. [\<C> ''as'' \<mapsto> \<up>(Msg (SenderBool x))]"
-  unfolding ubWell_def
+lift_definition createAsBundle :: "bool \<Rightarrow> senderMessage tsyn sbElem" is
+"\<lambda>x. [\<C> ''as'' \<mapsto> Msg (SenderBool x)]"
+  unfolding sbElemWell_def
   unfolding usclOkay_stream_def
   unfolding ctype_tsyn_def
   by simp
 
-lift_definition createIBundle :: "nat \<Rightarrow> senderMessage tsyn SB" is
-"\<lambda>x. [\<C> ''i'' \<mapsto> \<up>(Msg (SenderNat x))]"
-  unfolding ubWell_def
+lift_definition createIBundle :: "nat \<Rightarrow> senderMessage tsyn sbElem" is
+"\<lambda>x. [\<C> ''i'' \<mapsto> Msg (SenderNat x)]"
+  unfolding sbElemWell_def
   unfolding usclOkay_stream_def
   unfolding ctype_tsyn_def
   by simp
 
-lift_definition createDsBundle :: "(nat\<times>bool) \<Rightarrow> senderMessage tsyn SB" is
-"\<lambda>x. [\<C> ''ds'' \<mapsto> \<up>(Msg (SenderPair_SenderNat_SenderBool x))]"
-  unfolding ubWell_def
+lift_definition createDsBundle :: "(nat\<times>bool) \<Rightarrow> senderMessage tsyn sbElem" is
+"\<lambda>x. [\<C> ''ds'' \<mapsto> Msg (SenderPair_SenderNat_SenderBool x)]"
+  unfolding sbElemWell_def
   unfolding usclOkay_stream_def
   unfolding ctype_tsyn_def
   by simp
@@ -60,65 +60,68 @@ lift_definition createDsBundle :: "(nat\<times>bool) \<Rightarrow> senderMessage
 
 section \<open>Helpers to create a bundle from a single tsyn element\<close>
 
-fun createTsynAsBundle :: "bool tsyn \<Rightarrow> senderMessage tsyn SB" where
+fun createTsynAsBundle :: "bool tsyn \<Rightarrow> senderMessage tsyn sbElem" where
 "createTsynAsBundle (Msg x) = (createAsBundle x)" |
-"createTsynAsBundle null = (tsynbNull (\<C> ''as''))"
+"createTsynAsBundle null = (sbeNull {\<C> ''as''})"
 
-fun createTsynIBundle :: "nat tsyn \<Rightarrow> senderMessage tsyn SB" where
+fun createTsynIBundle :: "nat tsyn \<Rightarrow> senderMessage tsyn sbElem" where
 "createTsynIBundle (Msg x) = (createIBundle x)" |
-"createTsynIBundle null = (tsynbNull (\<C> ''i''))"
+"createTsynIBundle null = (sbeNull {\<C> ''i''})"
 
-fun createTsynDsBundle :: "(nat\<times>bool) tsyn \<Rightarrow> senderMessage tsyn SB" where
+fun createTsynDsBundle :: "(nat\<times>bool) tsyn \<Rightarrow> senderMessage tsyn sbElem" where
 "createTsynDsBundle (Msg x) = (createDsBundle x)" |
-"createTsynDsBundle null = (tsynbNull (\<C> ''ds''))"
+"createTsynDsBundle null = (sbeNull {\<C> ''ds''})"
 
 
 section \<open>Helpers to create a bundle from a tsyn list of elements\<close>
 
 fun createLongAsBundle :: "(bool tsyn) list \<Rightarrow> senderMessage tsyn SB" where
-"createLongAsBundle (x#xs) = ubConcEq (createTsynAsBundle x)\<cdot>(createLongAsBundle xs)" |
+"createLongAsBundle (x#xs) = ubConcEq (sbe2SB (createTsynAsBundle x))\<cdot>(createLongAsBundle xs)" |
 "createLongAsBundle []     = ubLeast {\<C> ''as''}"
 
 fun createLongIBundle :: "(nat tsyn) list \<Rightarrow> senderMessage tsyn SB" where
-"createLongIBundle (x#xs) = ubConcEq (createTsynIBundle x)\<cdot>(createLongIBundle xs)" |
+"createLongIBundle (x#xs) = ubConcEq (sbe2SB (createTsynIBundle x))\<cdot>(createLongIBundle xs)" |
 "createLongIBundle []     = ubLeast {\<C> ''i''}"
 
 fun createLongDsBundle :: "((nat\<times>bool) tsyn) list \<Rightarrow> senderMessage tsyn SB" where
-"createLongDsBundle (x#xs) = ubConcEq (createTsynDsBundle x)\<cdot>(createLongDsBundle xs)" |
+"createLongDsBundle (x#xs) = ubConcEq (sbe2SB (createTsynDsBundle x))\<cdot>(createLongDsBundle xs)" |
 "createLongDsBundle []     = ubLeast {\<C> ''ds''}"
 
 
 section \<open>Lemmas for "createXBundle"\<close>
 
-lemma createAsBundle_dom [simp]: "ubDom\<cdot>(createAsBundle x) = {\<C> ''as''}"
-  by (simp add: createAsBundle.rep_eq ubdom_insert)
+lemma createAsBundle_dom [simp]: "sbeDom (createAsBundle x) = {\<C> ''as''}"
+  apply(simp add: sbeDom_def createAsBundle_def)
+  using createAsBundle.abs_eq createAsBundle.rep_eq by auto
 
-lemma createAsBundle_getch [simp]: "(createAsBundle x).(\<C> ''as'') = \<up>(Msg (SenderBool x))"
-  by (simp add: createAsBundle.rep_eq ubgetch_insert)
+lemma createAsBundle_getch [simp]: "(sbe2SB (createAsBundle x)).(\<C> ''as'') = \<up>(Msg (SenderBool x))"
+  by (simp add: createAsBundle.rep_eq sbe2sb_getch)
 
-lemma createAsBundle_len [simp]: "ubLen (createAsBundle x) = Fin 1"
+lemma createAsBundle_len [simp]: "ubLen (sbe2SB (createAsBundle x)) = Fin 1"
   apply (subst ubLen_def)
   apply (simp add: usclLen_stream_def)
   by (metis (full_types) LeastI)
 
-lemma createIBundle_dom [simp]: "ubDom\<cdot>(createIBundle x) = {\<C> ''i''}"
-  by (simp add: createIBundle.rep_eq ubdom_insert)
+lemma createIBundle_dom [simp]: "sbeDom (createIBundle x) = {\<C> ''i''}"
+  apply(simp add: sbeDom_def createIBundle_def)
+  using createIBundle.abs_eq createIBundle.rep_eq by auto
 
-lemma createIBundle_getch [simp]: "(createIBundle x).(\<C> ''i'') = \<up>(Msg (SenderNat x))"
-  by (simp add: createIBundle.rep_eq ubgetch_insert)
+lemma createIBundle_getch [simp]: "(sbe2SB (createIBundle x)).(\<C> ''i'') = \<up>(Msg (SenderNat x))"
+  by (simp add: createIBundle.rep_eq sbe2sb_getch)
 
-lemma createIBundle_len [simp]: "ubLen (createIBundle x) = Fin 1"
+lemma createIBundle_len [simp]: "ubLen (sbe2SB (createIBundle x)) = Fin 1"
   apply (subst ubLen_def)
   apply (simp add: usclLen_stream_def)
   by (metis (full_types) LeastI)
 
-lemma createDsBundle_dom [simp]: "ubDom\<cdot>(createDsBundle x) = {\<C> ''ds''}"
-  by (simp add: createDsBundle.rep_eq ubdom_insert)
+lemma createDsBundle_dom [simp]: "sbeDom (createDsBundle x) = {\<C> ''ds''}"
+  apply(simp add: sbeDom_def createDsBundle_def)
+  using createDsBundle.abs_eq createDsBundle.rep_eq by auto
 
-lemma createDsBundle_getch [simp]: "(createDsBundle x).(\<C> ''ds'') = \<up>(Msg (SenderPair_SenderNat_SenderBool x))"
-  by (simp add: createDsBundle.rep_eq ubgetch_insert)
+lemma createDsBundle_getch [simp]: "(sbe2SB (createDsBundle x)).(\<C> ''ds'') = \<up>(Msg (SenderPair_SenderNat_SenderBool x))"
+  by (simp add: createDsBundle.rep_eq sbe2sb_getch)
 
-lemma createDsBundle_len [simp]: "ubLen (createDsBundle x) = Fin 1"
+lemma createDsBundle_len [simp]: "ubLen (sbe2SB (createDsBundle x)) = Fin 1"
   apply (subst ubLen_def)
   apply (simp add: usclLen_stream_def)
   by (metis (full_types) LeastI)
@@ -126,24 +129,24 @@ lemma createDsBundle_len [simp]: "ubLen (createDsBundle x) = Fin 1"
 
 section \<open>Lemmas for "createTsynXBundle"\<close>
 
-lemma createTsynAsBundle_dom [simp]: "ubDom\<cdot>(createTsynAsBundle x) = {\<C> ''as''}"
+lemma createTsynAsBundle_dom [simp]: "sbeDom (createTsynAsBundle x) = {\<C> ''as''}"
   by (cases x, simp_all)
 
-lemma createTsynAsBundle_len [simp]: "ubLen (createTsynAsBundle x) = Fin 1"
+lemma createTsynAsBundle_len [simp]: "ubLen (sbe2DB (createTsynAsBundle x)) = Fin 1"
   apply (cases x, simp_all)
   oops
 
-lemma createTsynIBundle_dom [simp]: "ubDom\<cdot>(createTsynIBundle x) = {\<C> ''i''}"
+lemma createTsynIBundle_dom [simp]: "sbeDom (createTsynIBundle x) = {\<C> ''i''}"
   by (cases x, simp_all)
 
-lemma createTsynIBundle_len [simp]: "ubLen (createTsynIBundle x) = Fin 1"
+lemma createTsynIBundle_len [simp]: "ubLen (sbe2DB (createTsynIBundle x)) = Fin 1"
   apply (cases x, simp_all)
   oops
 
-lemma createTsynDsBundle_dom [simp]: "ubDom\<cdot>(createTsynDsBundle x) = {\<C> ''ds''}"
+lemma createTsynDsBundle_dom [simp]: "sbeDom (createTsynDsBundle x) = {\<C> ''ds''}"
   by (cases x, simp_all)
 
-lemma createTsynDsBundle_len [simp]: "ubLen (createTsynDsBundle x) = Fin 1"
+lemma createTsynDsBundle_len [simp]: "ubLen (sbe2DB (createTsynDsBundle x)) = Fin 1"
   apply (cases x, simp_all)
   oops
 
@@ -222,70 +225,70 @@ fun getC :: "SenderState \<Rightarrow> nat" where
 (* Helper that allows us to utilize pattern matching *)
 fun senderTransitionH :: "(SenderState \<times> (senderMessage tsyn \<times> senderMessage tsyn)) \<Rightarrow> (SenderState \<times> senderMessage tsyn SB)" where
 "senderTransitionH (SenderState Sf var_buffer var_c, (\<^cancel>\<open>as\<mapsto>\<close>Msg (SenderBool port_as), \<^cancel>\<open>i\<mapsto>\<close>Msg (SenderNat port_i))) =
-  (if((size var_buffer)>1 \<and> port_as=False) then ((SenderState St (prepend (butlast var_buffer) port_i) 3, (createDsBundle (Pair (last (butlast var_buffer)) True))))
-   else if((size var_buffer)=1 \<and> port_as=False) then ((SenderState St (prepend (butlast var_buffer) port_i) 3, (createDsBundle (Pair port_i True))))
-   else if((size var_buffer)=0) then ((SenderState Sf (prepend var_buffer port_i) 3, (createDsBundle (Pair port_i False))))
+  (if((size var_buffer)>1 \<and> port_as=False) then ((SenderState St (prepend (butlast var_buffer) port_i) 3, (sbe2SB (createDsBundle (Pair (last (butlast var_buffer)) True)))))
+   else if((size var_buffer)=1 \<and> port_as=False) then ((SenderState St (prepend (butlast var_buffer) port_i) 3, (sbe2SB (createDsBundle (Pair port_i True)))))
+   else if((size var_buffer)=0) then ((SenderState Sf (prepend var_buffer port_i) 3, (sbe2SB (createDsBundle (Pair port_i False)))))
    else if((size var_buffer)>0 \<and> var_c>0 \<and> port_as=True) then ((SenderState Sf (prepend var_buffer port_i) (var_c-1), (tsynbNull (\<C> ''ds''))))
-   else if((size var_buffer)>0 \<and> var_c=0 \<and> port_as=True) then ((SenderState Sf (prepend var_buffer port_i) 3, (createDsBundle (Pair (last var_buffer) False))))
+   else if((size var_buffer)>0 \<and> var_c=0 \<and> port_as=True) then ((SenderState Sf (prepend var_buffer port_i) 3, (sbe2SB (createDsBundle (Pair (last var_buffer) False)))))
    else (SenderState Sf var_buffer var_c, (tsynbNull (\<C> ''ds''))))" |
 
 "senderTransitionH (SenderState Sf var_buffer var_c, (\<^cancel>\<open>as\<mapsto>\<close>Msg (SenderBool port_as), \<^cancel>\<open>i\<mapsto>\<close>null)) =
-  (if((size var_buffer)>1 \<and> port_as=False) then ((SenderState St (butlast var_buffer) 3, (createDsBundle (Pair (last (butlast var_buffer)) True))))
+  (if((size var_buffer)>1 \<and> port_as=False) then ((SenderState St (butlast var_buffer) 3, (sbe2SB (createDsBundle (Pair (last (butlast var_buffer)) True)))))
    else if((size var_buffer)=1 \<and> port_as=False) then ((SenderState St (butlast var_buffer) var_c, (tsynbNull (\<C> ''ds''))))
    else if((size var_buffer)=0) then ((SenderState Sf var_buffer var_c, (tsynbNull (\<C> ''ds''))))
    else if((size var_buffer)>0 \<and> var_c>0 \<and> port_as=True) then ((SenderState Sf var_buffer (var_c-1), (tsynbNull (\<C> ''ds''))))
-   else if((size var_buffer)>0 \<and> var_c=0 \<and> port_as=True) then ((SenderState Sf var_buffer 3, (createDsBundle (Pair (last var_buffer) False))))
+   else if((size var_buffer)>0 \<and> var_c=0 \<and> port_as=True) then ((SenderState Sf var_buffer 3, (sbe2SB (createDsBundle (Pair (last var_buffer) False)))))
    else (SenderState Sf var_buffer var_c, (tsynbNull (\<C> ''ds''))))" |
 
 "senderTransitionH (SenderState Sf var_buffer var_c, (\<^cancel>\<open>as\<mapsto>\<close>null, \<^cancel>\<open>i\<mapsto>\<close>Msg (SenderNat port_i))) =
-  (if((size var_buffer)=0) then ((SenderState Sf (prepend var_buffer port_i) 3, (createDsBundle (Pair port_i False))))
+  (if((size var_buffer)=0) then ((SenderState Sf (prepend var_buffer port_i) 3, (sbe2SB (createDsBundle (Pair port_i False)))))
    else if((size var_buffer)>0 \<and> var_c>0) then ((SenderState Sf (prepend var_buffer port_i) (var_c-1), (tsynbNull (\<C> ''ds''))))
-   else if((size var_buffer)>0 \<and> var_c=0) then ((SenderState Sf (prepend var_buffer port_i) 3, (createDsBundle (Pair (last var_buffer) False))))
+   else if((size var_buffer)>0 \<and> var_c=0) then ((SenderState Sf (prepend var_buffer port_i) 3, (sbe2SB (createDsBundle (Pair (last var_buffer) False)))))
    else (SenderState Sf var_buffer var_c, (tsynbNull (\<C> ''ds''))))" |
 
 "senderTransitionH (SenderState Sf var_buffer var_c, (\<^cancel>\<open>as\<mapsto>\<close>null, \<^cancel>\<open>i\<mapsto>\<close>null)) =
   (if((size var_buffer)=0) then ((SenderState Sf var_buffer var_c, (tsynbNull (\<C> ''ds''))))
    else if((size var_buffer)>0 \<and> var_c>0) then ((SenderState Sf var_buffer var_c, (tsynbNull (\<C> ''ds''))))
-   else if((size var_buffer)>0 \<and> var_c=0) then ((SenderState Sf var_buffer 3, (createDsBundle (Pair (last var_buffer) False))))
+   else if((size var_buffer)>0 \<and> var_c=0) then ((SenderState Sf var_buffer 3, (sbe2SB (createDsBundle (Pair (last var_buffer) False)))))
    else (SenderState Sf var_buffer var_c, (tsynbNull (\<C> ''ds''))))" |
 
 "senderTransitionH (SenderState St var_buffer var_c, (\<^cancel>\<open>as\<mapsto>\<close>Msg (SenderBool port_as), \<^cancel>\<open>i\<mapsto>\<close>Msg (SenderNat port_i))) =
-  (if((size var_buffer)=0) then ((SenderState St (prepend var_buffer port_i) 3, (createDsBundle (Pair port_i True))))
-   else if((size var_buffer)>1 \<and> port_as=True) then ((SenderState Sf (prepend (butlast var_buffer) port_i) 3, (createDsBundle (Pair (last (butlast var_buffer)) False))))
+  (if((size var_buffer)=0) then ((SenderState St (prepend var_buffer port_i) 3, (sbe2SB (createDsBundle (Pair port_i True)))))
+   else if((size var_buffer)>1 \<and> port_as=True) then ((SenderState Sf (prepend (butlast var_buffer) port_i) 3, (sbe2SB (createDsBundle (Pair (last (butlast var_buffer)) False)))))
    else if((size var_buffer)>0 \<and> var_c>0 \<and> port_as=False) then ((SenderState St (prepend var_buffer port_i) (var_c-1), (tsynbNull (\<C> ''ds''))))
-   else if((size var_buffer)>0 \<and> var_c=0 \<and> port_as=False) then ((SenderState St (prepend var_buffer port_i) 3, (createDsBundle (Pair (last var_buffer) True))))
-   else if((size var_buffer)=1 \<and> port_as=True) then ((SenderState Sf (prepend (butlast var_buffer) port_i) 3, (createDsBundle (Pair port_i False))))
+   else if((size var_buffer)>0 \<and> var_c=0 \<and> port_as=False) then ((SenderState St (prepend var_buffer port_i) 3, (sbe2SB (createDsBundle (Pair (last var_buffer) True)))))
+   else if((size var_buffer)=1 \<and> port_as=True) then ((SenderState Sf (prepend (butlast var_buffer) port_i) 3, (sbe2SB (createDsBundle (Pair port_i False)))))
    else (SenderState St var_buffer var_c, (tsynbNull (\<C> ''ds''))))" |
 
 "senderTransitionH (SenderState St var_buffer var_c, (\<^cancel>\<open>as\<mapsto>\<close>Msg (SenderBool port_as), \<^cancel>\<open>i\<mapsto>\<close>null)) =
   (if((size var_buffer)=0) then ((SenderState St var_buffer var_c, (tsynbNull (\<C> ''ds''))))
-   else if((size var_buffer)>1 \<and> port_as=True) then ((SenderState Sf (butlast var_buffer) 3, (createDsBundle (Pair (last (butlast var_buffer)) False))))
+   else if((size var_buffer)>1 \<and> port_as=True) then ((SenderState Sf (butlast var_buffer) 3, (sbe2SB (createDsBundle (Pair (last (butlast var_buffer)) False)))))
    else if((size var_buffer)>0 \<and> var_c>0 \<and> port_as=False) then ((SenderState St var_buffer (var_c-1), (tsynbNull (\<C> ''ds''))))
-   else if((size var_buffer)>0 \<and> var_c=0 \<and> port_as=False) then ((SenderState St var_buffer 3, (createDsBundle (Pair (last var_buffer) True))))
+   else if((size var_buffer)>0 \<and> var_c=0 \<and> port_as=False) then ((SenderState St var_buffer 3, (sbe2SB (createDsBundle (Pair (last var_buffer) True)))))
    else if((size var_buffer)=1 \<and> port_as=True) then ((SenderState Sf (butlast var_buffer) var_c, (tsynbNull (\<C> ''ds''))))
    else (SenderState St var_buffer var_c, (tsynbNull (\<C> ''ds''))))" |
 
 "senderTransitionH (SenderState St var_buffer var_c, (\<^cancel>\<open>as\<mapsto>\<close>null, \<^cancel>\<open>i\<mapsto>\<close>Msg (SenderNat port_i))) =
-  (if((size var_buffer)=0) then ((SenderState St (prepend var_buffer port_i) 3, (createDsBundle (Pair port_i True))))
+  (if((size var_buffer)=0) then ((SenderState St (prepend var_buffer port_i) 3, (sbe2SB (createDsBundle (Pair port_i True)))))
    else if((size var_buffer)>0 \<and> var_c>0) then ((SenderState St (prepend var_buffer port_i) (var_c-1), (tsynbNull (\<C> ''ds''))))
-   else if((size var_buffer)>0 \<and> var_c=0) then ((SenderState St (prepend var_buffer port_i) 3, (createDsBundle (Pair (last var_buffer) True))))
+   else if((size var_buffer)>0 \<and> var_c=0) then ((SenderState St (prepend var_buffer port_i) 3, (sbe2SB (createDsBundle (Pair (last var_buffer) True)))))
    else (SenderState St var_buffer var_c, (tsynbNull (\<C> ''ds''))))" |
 
 "senderTransitionH (SenderState St var_buffer var_c, (\<^cancel>\<open>as\<mapsto>\<close>null, \<^cancel>\<open>i\<mapsto>\<close>null)) =
   (if((size var_buffer)=0) then ((SenderState St var_buffer var_c, (tsynbNull (\<C> ''ds''))))
    else if((size var_buffer)>0 \<and> var_c>0) then ((SenderState St var_buffer (var_c-1), (tsynbNull (\<C> ''ds''))))
-   else if((size var_buffer)>0 \<and> var_c=0) then ((SenderState St var_buffer 3, (createDsBundle (Pair (last var_buffer) True))))
+   else if((size var_buffer)>0 \<and> var_c=0) then ((SenderState St var_buffer 3, (sbe2SB (createDsBundle (Pair (last var_buffer) True)))))
    else (SenderState St var_buffer var_c, (tsynbNull (\<C> ''ds''))))"
 
 (* Transition function *)
 fun senderTransition :: "(SenderState \<times> senderMessage tsyn sbElem) \<Rightarrow> (SenderState \<times> senderMessage tsyn SB)" where
-"senderTransition (s,b) = (if dom(Rep_sbElem b) = {\<C> ''as'', \<C> ''i''} then senderTransitionH (s, (Rep_sbElem b\<rightharpoonup>\<C> ''as'', Rep_sbElem b\<rightharpoonup>\<C> ''i'')) else undefined)"
+"senderTransition (s,b) = (if (sbeDom b) = {\<C> ''as'', \<C> ''i''} then senderTransitionH (s, (Rep_sbElem b\<rightharpoonup>\<C> ''as'', Rep_sbElem b\<rightharpoonup>\<C> ''i'')) else undefined)"
 
 lift_definition SenderAutomaton :: "(SenderState, senderMessage tsyn) dAutomaton" is
 "(senderTransition, SenderState St []  0, tsynbNull (\<C> ''ds''), {\<C> ''as'', \<C> ''i''}, {\<C> ''ds''})"
   by simp
 
-definition SenderSPF :: "senderMessage tsyn SPF" where
+definition SenderSPF :: "(senderMessage tsyn, senderMessage tsyn) SPF" where
 "SenderSPF = da_H SenderAutomaton"
 
 
@@ -294,92 +297,92 @@ section \<open>Lemmata for the transitions\<close>
 (* Line 33 in the MAA model *)
 lemma tbd_0_0:
   assumes "(size var_buffer)>1 \<and> port_as=False"
-    shows "spfConcIn  (createAsBundle port_as \<uplus> createIBundle port_i)\<cdot>(da_h SenderAutomaton (SenderState Sf var_buffer var_c))
-         = spfConcOut (createDsBundle (Pair (last (butlast var_buffer)) True))\<cdot>(da_h SenderAutomaton (SenderState St (prepend (butlast var_buffer) port_i) 3))"
+    shows "spfConcIn  (sbe2DB (createAsBundle port_as) \<uplus> sbe2SB (createIBundle port_i))\<cdot>(da_h SenderAutomaton (SenderState Sf var_buffer var_c))
+         = spfConcOut (sbe2SB (createDsBundle (Pair (last (butlast var_buffer)) True)))\<cdot>(da_h SenderAutomaton (SenderState St (prepend (butlast var_buffer) port_i) 3))"
   oops
 
 (* Line 35 in the MAA model *)
 lemma tbd_0_1:
   assumes "(size var_buffer)=1 \<and> port_as=False"
-    shows "spfConcIn  (createAsBundle port_as \<uplus> createIBundle port_i)\<cdot>(da_h SenderAutomaton (SenderState Sf var_buffer var_c))
-         = spfConcOut (createDsBundle (Pair port_i True))\<cdot>(da_h SenderAutomaton (SenderState St (prepend (butlast var_buffer) port_i) 3))"
+    shows "spfConcIn  (sbe2DB (createAsBundle port_as) \<uplus> sbe2SB (createIBundle port_i))\<cdot>(da_h SenderAutomaton (SenderState Sf var_buffer var_c))
+         = spfConcOut (sbe2SB (createDsBundle (Pair port_i True)))\<cdot>(da_h SenderAutomaton (SenderState St (prepend (butlast var_buffer) port_i) 3))"
   oops
 
 (* Line 43 in the MAA model *)
 lemma tbd_0_2:
   assumes "(size var_buffer)=0"
-    shows "spfConcIn  (createAsBundle port_as \<uplus> createIBundle port_i)\<cdot>(da_h SenderAutomaton (SenderState Sf var_buffer var_c))
-         = spfConcOut (createDsBundle (Pair port_i False))\<cdot>(da_h SenderAutomaton (SenderState Sf (prepend var_buffer port_i) 3))"
+    shows "spfConcIn  (sbe2SB (createAsBundle port_as) \<uplus> sbe2SB (createIBundle port_i))\<cdot>(da_h SenderAutomaton (SenderState Sf var_buffer var_c))
+         = spfConcOut (sbe2SB (createDsBundle (Pair port_i False)))\<cdot>(da_h SenderAutomaton (SenderState Sf (prepend var_buffer port_i) 3))"
   oops
 
 (* Line 45 in the MAA model *)
 lemma tbd_0_3:
   assumes "(size var_buffer)>0 \<and> var_c>0 \<and> port_as=True"
-    shows "spfConcIn  (createAsBundle port_as \<uplus> createIBundle port_i)\<cdot>(da_h SenderAutomaton (SenderState Sf var_buffer var_c))
+    shows "spfConcIn  (sbe2DB (createAsBundle port_as) \<uplus> sbe2SB (createIBundle port_i))\<cdot>(da_h SenderAutomaton (SenderState Sf var_buffer var_c))
          = spfConcOut (tsynbNull (\<C> ''ds''))\<cdot>(da_h SenderAutomaton (SenderState Sf (prepend var_buffer port_i) (var_c-1)))"
   oops
 
 (* Line 47 in the MAA model *)
 lemma tbd_0_4:
   assumes "(size var_buffer)>0 \<and> var_c=0 \<and> port_as=True"
-    shows "spfConcIn  (createAsBundle port_as \<uplus> createIBundle port_i)\<cdot>(da_h SenderAutomaton (SenderState Sf var_buffer var_c))
-         = spfConcOut (createDsBundle (Pair (last var_buffer) False))\<cdot>(da_h SenderAutomaton (SenderState Sf (prepend var_buffer port_i) 3))"
+    shows "spfConcIn  (sbe2DB (createAsBundle port_as) \<uplus> sbe2SB (createIBundle port_i))\<cdot>(da_h SenderAutomaton (SenderState Sf var_buffer var_c))
+         = spfConcOut (sbe2SB (createDsBundle (Pair (last var_buffer) False)))\<cdot>(da_h SenderAutomaton (SenderState Sf (prepend var_buffer port_i) 3))"
   oops
 
 (* Line 34 in the MAA model *)
 lemma tbd_1_0:
   assumes "(size var_buffer)>1 \<and> port_as=False"
-    shows "spfConcIn  (createAsBundle port_as \<uplus> tsynbNull (\<C> ''i''))\<cdot>(da_h SenderAutomaton (SenderState Sf var_buffer var_c))
-         = spfConcOut (createDsBundle (Pair (last (butlast var_buffer)) True))\<cdot>(da_h SenderAutomaton (SenderState St (butlast var_buffer) 3))"
+    shows "spfConcIn  (sbe2DB (createAsBundle port_as) \<uplus> tsynbNull (\<C> ''i''))\<cdot>(da_h SenderAutomaton (SenderState Sf var_buffer var_c))
+         = spfConcOut (sbe2SB (createDsBundle (Pair (last (butlast var_buffer)) True)))\<cdot>(da_h SenderAutomaton (SenderState St (butlast var_buffer) 3))"
   oops
 
 (* Line 36 in the MAA model *)
 lemma tbd_1_1:
   assumes "(size var_buffer)=1 \<and> port_as=False"
-    shows "spfConcIn  (createAsBundle port_as \<uplus> tsynbNull (\<C> ''i''))\<cdot>(da_h SenderAutomaton (SenderState Sf var_buffer var_c))
+    shows "spfConcIn  (sbe2DB (createAsBundle port_as) \<uplus> tsynbNull (\<C> ''i''))\<cdot>(da_h SenderAutomaton (SenderState Sf var_buffer var_c))
          = spfConcOut (tsynbNull (\<C> ''ds''))\<cdot>(da_h SenderAutomaton (SenderState St (butlast var_buffer) var_c))"
   oops
 
 (* Line 38 in the MAA model *)
 lemma tbd_1_2:
   assumes "(size var_buffer)=0"
-    shows "spfConcIn  (createAsBundle port_as \<uplus> tsynbNull (\<C> ''i''))\<cdot>(da_h SenderAutomaton (SenderState Sf var_buffer var_c))
+    shows "spfConcIn  (sbe2SB (createAsBundle port_as) \<uplus> tsynbNull (\<C> ''i''))\<cdot>(da_h SenderAutomaton (SenderState Sf var_buffer var_c))
          = spfConcOut (tsynbNull (\<C> ''ds''))\<cdot>(da_h SenderAutomaton (SenderState Sf var_buffer var_c))"
   oops
 
 (* Line 40 in the MAA model *)
 lemma tbd_1_3:
   assumes "(size var_buffer)>0 \<and> var_c>0 \<and> port_as=True"
-    shows "spfConcIn  (createAsBundle port_as \<uplus> tsynbNull (\<C> ''i''))\<cdot>(da_h SenderAutomaton (SenderState Sf var_buffer var_c))
+    shows "spfConcIn  (sbe2DB (createAsBundle port_as) \<uplus> tsynbNull (\<C> ''i''))\<cdot>(da_h SenderAutomaton (SenderState Sf var_buffer var_c))
          = spfConcOut (tsynbNull (\<C> ''ds''))\<cdot>(da_h SenderAutomaton (SenderState Sf var_buffer (var_c-1)))"
   oops
 
 (* Line 41 in the MAA model *)
 lemma tbd_1_4:
   assumes "(size var_buffer)>0 \<and> var_c=0 \<and> port_as=True"
-    shows "spfConcIn  (createAsBundle port_as \<uplus> tsynbNull (\<C> ''i''))\<cdot>(da_h SenderAutomaton (SenderState Sf var_buffer var_c))
-         = spfConcOut (createDsBundle (Pair (last var_buffer) False))\<cdot>(da_h SenderAutomaton (SenderState Sf var_buffer 3))"
+    shows "spfConcIn  (sbe2DB (createAsBundle port_as) \<uplus> tsynbNull (\<C> ''i''))\<cdot>(da_h SenderAutomaton (SenderState Sf var_buffer var_c))
+         = spfConcOut (sbe2SB (createDsBundle (Pair (last var_buffer) False)))\<cdot>(da_h SenderAutomaton (SenderState Sf var_buffer 3))"
   oops
 
 (* Line 44 in the MAA model *)
 lemma tbd_2_0:
   assumes "(size var_buffer)=0"
-    shows "spfConcIn  (tsynbNull (\<C> ''as'') \<uplus> createIBundle port_i)\<cdot>(da_h SenderAutomaton (SenderState Sf var_buffer var_c))
-         = spfConcOut (createDsBundle (Pair port_i False))\<cdot>(da_h SenderAutomaton (SenderState Sf (prepend var_buffer port_i) 3))"
+    shows "spfConcIn  (tsynbNull (\<C> ''as'') \<uplus> sbe2SB (createIBundle port_i))\<cdot>(da_h SenderAutomaton (SenderState Sf var_buffer var_c))
+         = spfConcOut (sbe2SB (createDsBundle (Pair port_i False)))\<cdot>(da_h SenderAutomaton (SenderState Sf (prepend var_buffer port_i) 3))"
   oops
 
 (* Line 46 in the MAA model *)
 lemma tbd_2_1:
   assumes "(size var_buffer)>0 \<and> var_c>0"
-    shows "spfConcIn  (tsynbNull (\<C> ''as'') \<uplus> createIBundle port_i)\<cdot>(da_h SenderAutomaton (SenderState Sf var_buffer var_c))
+    shows "spfConcIn  (tsynbNull (\<C> ''as'') \<uplus> sbe2SB (createIBundle port_i))\<cdot>(da_h SenderAutomaton (SenderState Sf var_buffer var_c))
          = spfConcOut (tsynbNull (\<C> ''ds''))\<cdot>(da_h SenderAutomaton (SenderState Sf (prepend var_buffer port_i) (var_c-1)))"
   oops
 
 (* Line 48 in the MAA model *)
 lemma tbd_2_2:
   assumes "(size var_buffer)>0 \<and> var_c=0"
-    shows "spfConcIn  (tsynbNull (\<C> ''as'') \<uplus> createIBundle port_i)\<cdot>(da_h SenderAutomaton (SenderState Sf var_buffer var_c))
-         = spfConcOut (createDsBundle (Pair (last var_buffer) False))\<cdot>(da_h SenderAutomaton (SenderState Sf (prepend var_buffer port_i) 3))"
+    shows "spfConcIn  (tsynbNull (\<C> ''as'') \<uplus> sbe2SB (createIBundle port_i))\<cdot>(da_h SenderAutomaton (SenderState Sf var_buffer var_c))
+         = spfConcOut (sbe2SB (createDsBundle (Pair (last var_buffer) False)))\<cdot>(da_h SenderAutomaton (SenderState Sf (prepend var_buffer port_i) 3))"
   oops
 
 (* Line 37 in the MAA model *)
@@ -400,98 +403,98 @@ lemma tbd_3_1:
 lemma tbd_3_2:
   assumes "(size var_buffer)>0 \<and> var_c=0"
     shows "spfConcIn  (tsynbNull (\<C> ''as'') \<uplus> tsynbNull (\<C> ''i''))\<cdot>(da_h SenderAutomaton (SenderState Sf var_buffer var_c))
-         = spfConcOut (createDsBundle (Pair (last var_buffer) False))\<cdot>(da_h SenderAutomaton (SenderState Sf var_buffer 3))"
+         = spfConcOut (sbe2SB (createDsBundle (Pair (last var_buffer) False)))\<cdot>(da_h SenderAutomaton (SenderState Sf var_buffer 3))"
   oops
 
 (* Line 25 in the MAA model *)
 lemma tbd_4_0:
   assumes "(size var_buffer)=0"
-    shows "spfConcIn  (createAsBundle port_as \<uplus> createIBundle port_i)\<cdot>(da_h SenderAutomaton (SenderState St var_buffer var_c))
-         = spfConcOut (createDsBundle (Pair port_i True))\<cdot>(da_h SenderAutomaton (SenderState St (prepend var_buffer port_i) 3))"
+    shows "spfConcIn  (sbe2SB (createAsBundle port_as) \<uplus> sbe2SB (createIBundle port_i))\<cdot>(da_h SenderAutomaton (SenderState St var_buffer var_c))
+         = spfConcOut (sbe2SB (createDsBundle (Pair port_i True)))\<cdot>(da_h SenderAutomaton (SenderState St (prepend var_buffer port_i) 3))"
   oops
 
 (* Line 27 in the MAA model *)
 lemma tbd_4_1:
   assumes "(size var_buffer)>1 \<and> port_as=True"
-    shows "spfConcIn  (createAsBundle port_as \<uplus> createIBundle port_i)\<cdot>(da_h SenderAutomaton (SenderState St var_buffer var_c))
-         = spfConcOut (createDsBundle (Pair (last (butlast var_buffer)) False))\<cdot>(da_h SenderAutomaton (SenderState Sf (prepend (butlast var_buffer) port_i) 3))"
+    shows "spfConcIn  (sbe2DB (createAsBundle port_as) \<uplus> sbe2SB (createIBundle port_i))\<cdot>(da_h SenderAutomaton (SenderState St var_buffer var_c))
+         = spfConcOut (sbe2SB (createDsBundle (Pair (last (butlast var_buffer)) False)))\<cdot>(da_h SenderAutomaton (SenderState Sf (prepend (butlast var_buffer) port_i) 3))"
   oops
 
 (* Line 28 in the MAA model *)
 lemma tbd_4_2:
   assumes "(size var_buffer)>0 \<and> var_c>0 \<and> port_as=False"
-    shows "spfConcIn  (createAsBundle port_as \<uplus> createIBundle port_i)\<cdot>(da_h SenderAutomaton (SenderState St var_buffer var_c))
+    shows "spfConcIn  (sbe2DB (createAsBundle port_as) \<uplus> sbe2SB (createIBundle port_i))\<cdot>(da_h SenderAutomaton (SenderState St var_buffer var_c))
          = spfConcOut (tsynbNull (\<C> ''ds''))\<cdot>(da_h SenderAutomaton (SenderState St (prepend var_buffer port_i) (var_c-1)))"
   oops
 
 (* Line 30 in the MAA model *)
 lemma tbd_4_3:
   assumes "(size var_buffer)>0 \<and> var_c=0 \<and> port_as=False"
-    shows "spfConcIn  (createAsBundle port_as \<uplus> createIBundle port_i)\<cdot>(da_h SenderAutomaton (SenderState St var_buffer var_c))
-         = spfConcOut (createDsBundle (Pair (last var_buffer) True))\<cdot>(da_h SenderAutomaton (SenderState St (prepend var_buffer port_i) 3))"
+    shows "spfConcIn  (sbe2DB (createAsBundle port_as) \<uplus> sbe2SB (createIBundle port_i))\<cdot>(da_h SenderAutomaton (SenderState St var_buffer var_c))
+         = spfConcOut (sbe2SB (createDsBundle (Pair (last var_buffer) True)))\<cdot>(da_h SenderAutomaton (SenderState St (prepend var_buffer port_i) 3))"
   oops
 
 (* Line 32 in the MAA model *)
 lemma tbd_4_4:
   assumes "(size var_buffer)=1 \<and> port_as=True"
-    shows "spfConcIn  (createAsBundle port_as \<uplus> createIBundle port_i)\<cdot>(da_h SenderAutomaton (SenderState St var_buffer var_c))
-         = spfConcOut (createDsBundle (Pair port_i False))\<cdot>(da_h SenderAutomaton (SenderState Sf (prepend (butlast var_buffer) port_i) 3))"
+    shows "spfConcIn  (sbe2DB (createAsBundle port_as) \<uplus> sbe2SB (createIBundle port_i))\<cdot>(da_h SenderAutomaton (SenderState St var_buffer var_c))
+         = spfConcOut (sbe2SB (createDsBundle (Pair port_i False)))\<cdot>(da_h SenderAutomaton (SenderState Sf (prepend (butlast var_buffer) port_i) 3))"
   oops
 
 (* Line 17 in the MAA model *)
 lemma tbd_5_0:
   assumes "(size var_buffer)=0"
-    shows "spfConcIn  (createAsBundle port_as \<uplus> tsynbNull (\<C> ''i''))\<cdot>(da_h SenderAutomaton (SenderState St var_buffer var_c))
+    shows "spfConcIn  (sbe2SB (createAsBundle port_as) \<uplus> tsynbNull (\<C> ''i''))\<cdot>(da_h SenderAutomaton (SenderState St var_buffer var_c))
          = spfConcOut (tsynbNull (\<C> ''ds''))\<cdot>(da_h SenderAutomaton (SenderState St var_buffer var_c))"
   oops
 
 (* Line 18 in the MAA model *)
 lemma tbd_5_1:
   assumes "(size var_buffer)>1 \<and> port_as=True"
-    shows "spfConcIn  (createAsBundle port_as \<uplus> tsynbNull (\<C> ''i''))\<cdot>(da_h SenderAutomaton (SenderState St var_buffer var_c))
-         = spfConcOut (createDsBundle (Pair (last (butlast var_buffer)) False))\<cdot>(da_h SenderAutomaton (SenderState Sf (butlast var_buffer) 3))"
+    shows "spfConcIn  (sbe2DB (createAsBundle port_as) \<uplus> tsynbNull (\<C> ''i''))\<cdot>(da_h SenderAutomaton (SenderState St var_buffer var_c))
+         = spfConcOut (sbe2SB (createDsBundle (Pair (last (butlast var_buffer)) False)))\<cdot>(da_h SenderAutomaton (SenderState Sf (butlast var_buffer) 3))"
   oops
 
 (* Line 20 in the MAA model *)
 lemma tbd_5_2:
   assumes "(size var_buffer)>0 \<and> var_c>0 \<and> port_as=False"
-    shows "spfConcIn  (createAsBundle port_as \<uplus> tsynbNull (\<C> ''i''))\<cdot>(da_h SenderAutomaton (SenderState St var_buffer var_c))
+    shows "spfConcIn  (sbe2DB (createAsBundle port_as) \<uplus> tsynbNull (\<C> ''i''))\<cdot>(da_h SenderAutomaton (SenderState St var_buffer var_c))
          = spfConcOut (tsynbNull (\<C> ''ds''))\<cdot>(da_h SenderAutomaton (SenderState St var_buffer (var_c-1)))"
   oops
 
 (* Line 22 in the MAA model *)
 lemma tbd_5_3:
   assumes "(size var_buffer)>0 \<and> var_c=0 \<and> port_as=False"
-    shows "spfConcIn  (createAsBundle port_as \<uplus> tsynbNull (\<C> ''i''))\<cdot>(da_h SenderAutomaton (SenderState St var_buffer var_c))
-         = spfConcOut (createDsBundle (Pair (last var_buffer) True))\<cdot>(da_h SenderAutomaton (SenderState St var_buffer 3))"
+    shows "spfConcIn  (sbe2DB (createAsBundle port_as) \<uplus> tsynbNull (\<C> ''i''))\<cdot>(da_h SenderAutomaton (SenderState St var_buffer var_c))
+         = spfConcOut (sbe2SB (createDsBundle (Pair (last var_buffer) True)))\<cdot>(da_h SenderAutomaton (SenderState St var_buffer 3))"
   oops
 
 (* Line 24 in the MAA model *)
 lemma tbd_5_4:
   assumes "(size var_buffer)=1 \<and> port_as=True"
-    shows "spfConcIn  (createAsBundle port_as \<uplus> tsynbNull (\<C> ''i''))\<cdot>(da_h SenderAutomaton (SenderState St var_buffer var_c))
+    shows "spfConcIn  (sbe2DB (createAsBundle port_as) \<uplus> tsynbNull (\<C> ''i''))\<cdot>(da_h SenderAutomaton (SenderState St var_buffer var_c))
          = spfConcOut (tsynbNull (\<C> ''ds''))\<cdot>(da_h SenderAutomaton (SenderState Sf (butlast var_buffer) var_c))"
   oops
 
 (* Line 26 in the MAA model *)
 lemma tbd_6_0:
   assumes "(size var_buffer)=0"
-    shows "spfConcIn  (tsynbNull (\<C> ''as'') \<uplus> createIBundle port_i)\<cdot>(da_h SenderAutomaton (SenderState St var_buffer var_c))
-         = spfConcOut (createDsBundle (Pair port_i True))\<cdot>(da_h SenderAutomaton (SenderState St (prepend var_buffer port_i) 3))"
+    shows "spfConcIn  (tsynbNull (\<C> ''as'') \<uplus> sbe2SB (createIBundle port_i))\<cdot>(da_h SenderAutomaton (SenderState St var_buffer var_c))
+         = spfConcOut (sbe2SB (createDsBundle (Pair port_i True)))\<cdot>(da_h SenderAutomaton (SenderState St (prepend var_buffer port_i) 3))"
   oops
 
 (* Line 29 in the MAA model *)
 lemma tbd_6_1:
   assumes "(size var_buffer)>0 \<and> var_c>0"
-    shows "spfConcIn  (tsynbNull (\<C> ''as'') \<uplus> createIBundle port_i)\<cdot>(da_h SenderAutomaton (SenderState St var_buffer var_c))
+    shows "spfConcIn  (tsynbNull (\<C> ''as'') \<uplus> sbe2SB (createIBundle port_i))\<cdot>(da_h SenderAutomaton (SenderState St var_buffer var_c))
          = spfConcOut (tsynbNull (\<C> ''ds''))\<cdot>(da_h SenderAutomaton (SenderState St (prepend var_buffer port_i) (var_c-1)))"
   oops
 
 (* Line 31 in the MAA model *)
 lemma tbd_6_2:
   assumes "(size var_buffer)>0 \<and> var_c=0"
-    shows "spfConcIn  (tsynbNull (\<C> ''as'') \<uplus> createIBundle port_i)\<cdot>(da_h SenderAutomaton (SenderState St var_buffer var_c))
-         = spfConcOut (createDsBundle (Pair (last var_buffer) True))\<cdot>(da_h SenderAutomaton (SenderState St (prepend var_buffer port_i) 3))"
+    shows "spfConcIn  (tsynbNull (\<C> ''as'') \<uplus> sbe2SB (createIBundle port_i))\<cdot>(da_h SenderAutomaton (SenderState St var_buffer var_c))
+         = spfConcOut (sbe2SB (createDsBundle (Pair (last var_buffer) True)))\<cdot>(da_h SenderAutomaton (SenderState St (prepend var_buffer port_i) 3))"
   oops
 
 (* Line 19 in the MAA model *)
@@ -512,7 +515,7 @@ lemma tbd_7_1:
 lemma tbd_7_2:
   assumes "(size var_buffer)>0 \<and> var_c=0"
     shows "spfConcIn  (tsynbNull (\<C> ''as'') \<uplus> tsynbNull (\<C> ''i''))\<cdot>(da_h SenderAutomaton (SenderState St var_buffer var_c))
-         = spfConcOut (createDsBundle (Pair (last var_buffer) True))\<cdot>(da_h SenderAutomaton (SenderState St var_buffer 3))"
+         = spfConcOut (sbe2SB (createDsBundle (Pair (last var_buffer) True)))\<cdot>(da_h SenderAutomaton (SenderState St var_buffer 3))"
   oops
 
 
